fix Tag spec, add integer spec, test bool correctness proof

src/INTEGER.light.c
@@ -1,0 +1,2874 @@
+struct asn_codec_ctx_s;
+struct asn_enc_rval_s;
+struct asn_dec_rval_s;
+struct asn_bit_data_s;
+struct asn_bit_outp_s;
+struct asn_per_constraint_s;
+struct asn_per_constraints_s;
+struct asn_random_fill_result_s;
+struct asn_oer_constraint_number_s;
+struct asn_oer_constraints_s;
+struct asn_type_selector_result_s;
+struct asn_TYPE_operation_s;
+struct asn_encoding_constraints_s;
+struct asn_TYPE_descriptor_s;
+struct asn_TYPE_member_s;
+struct ASN__PRIMITIVE_TYPE_s;
+struct asn_INTEGER_enum_map_s;
+struct asn_INTEGER_specifics_s;
+union _2079;
+struct e2v_key;
+struct asn_codec_ctx_s {
+  unsigned int max_stack_size;
+};
+
+struct asn_enc_rval_s {
+  int encoded;
+  struct asn_TYPE_descriptor_s *failed_type;
+  void *structure_ptr;
+};
+
+struct asn_dec_rval_s {
+  int code;
+  unsigned int consumed;
+};
+
+struct asn_bit_data_s {
+  unsigned char *buffer;
+  unsigned int nboff;
+  unsigned int nbits;
+  unsigned int moved;
+  int (*refill)(struct asn_bit_data_s *);
+  void *refill_key;
+};
+
+struct asn_bit_outp_s {
+  unsigned char *buffer;
+  unsigned int nboff;
+  unsigned int nbits;
+  unsigned char tmpspace[32];
+  int (*output)(void *, unsigned int, void *);
+  void *op_key;
+  unsigned int flushed_bytes;
+};
+
+struct asn_per_constraint_s {
+  int flags;
+  int range_bits;
+  int effective_bits;
+  int lower_bound;
+  int upper_bound;
+};
+
+struct asn_per_constraints_s {
+  struct asn_per_constraint_s value;
+  struct asn_per_constraint_s size;
+  int (*value2code)(unsigned int);
+  int (*code2value)(unsigned int);
+};
+
+struct asn_random_fill_result_s {
+  int code;
+  unsigned int length;
+};
+
+struct asn_oer_constraint_number_s {
+  unsigned int width;
+  unsigned int positive;
+};
+
+struct asn_oer_constraints_s {
+  struct asn_oer_constraint_number_s value;
+  int size;
+};
+
+struct asn_type_selector_result_s {
+  struct asn_TYPE_descriptor_s *type_descriptor;
+  unsigned int presence_index;
+};
+
+struct asn_TYPE_operation_s {
+  void (*free_struct)(struct asn_TYPE_descriptor_s *, void *, int);
+  int (*print_struct)(struct asn_TYPE_descriptor_s *, void *, int, int (*)(void *, unsigned int, void *), void *);
+  int (*compare_struct)(struct asn_TYPE_descriptor_s *, void *, void *);
+  void (*ber_decoder)(struct asn_dec_rval_s *, struct asn_codec_ctx_s *, struct asn_TYPE_descriptor_s *, void **, void *, unsigned int, int);
+  void (*der_encoder)(struct asn_enc_rval_s *, struct asn_TYPE_descriptor_s *, void *, int, unsigned int, int (*)(void *, unsigned int, void *), void *);
+  void (*xer_decoder)(struct asn_dec_rval_s *, struct asn_codec_ctx_s *, struct asn_TYPE_descriptor_s *, void **, signed char *, void *, unsigned int);
+  void (*xer_encoder)(struct asn_enc_rval_s *, struct asn_TYPE_descriptor_s *, void *, int, int, int (*)(void *, unsigned int, void *), void *);
+  void (*oer_decoder)(struct asn_dec_rval_s *, struct asn_codec_ctx_s *, struct asn_TYPE_descriptor_s *, struct asn_oer_constraints_s *, void **, void *, unsigned int);
+  void (*oer_encoder)(struct asn_enc_rval_s *, struct asn_TYPE_descriptor_s *, struct asn_oer_constraints_s *, void *, int (*)(void *, unsigned int, void *), void *);
+  void (*uper_decoder)(struct asn_dec_rval_s *, struct asn_codec_ctx_s *, struct asn_TYPE_descriptor_s *, struct asn_per_constraints_s *, void **, struct asn_bit_data_s *);
+  void (*uper_encoder)(struct asn_enc_rval_s *, struct asn_TYPE_descriptor_s *, struct asn_per_constraints_s *, void *, struct asn_bit_outp_s *);
+  void (*random_fill)(struct asn_random_fill_result_s *, struct asn_TYPE_descriptor_s *, void **, struct asn_encoding_constraints_s *, unsigned int);
+  unsigned int (*outmost_tag)(struct asn_TYPE_descriptor_s *, void *, int, unsigned int);
+};
+
+struct asn_encoding_constraints_s {
+  struct asn_oer_constraints_s *oer_constraints;
+  struct asn_per_constraints_s *per_constraints;
+  int (*general_constraints)(struct asn_TYPE_descriptor_s *, void *, void (*)(void *, struct asn_TYPE_descriptor_s *, void *, signed char *, ...), void *);
+};
+
+struct asn_TYPE_descriptor_s {
+  signed char *name;
+  signed char *xml_tag;
+  struct asn_TYPE_operation_s *op;
+  unsigned int *tags;
+  unsigned int tags_count;
+  unsigned int *all_tags;
+  unsigned int all_tags_count;
+  struct asn_encoding_constraints_s encoding_constraints;
+  struct asn_TYPE_member_s *elements;
+  unsigned int elements_count;
+  void *specifics;
+};
+
+struct asn_TYPE_member_s {
+  int flags;
+  unsigned int optional;
+  unsigned int memb_offset;
+  unsigned int tag;
+  int tag_mode;
+  struct asn_TYPE_descriptor_s *type;
+  void (*type_selector)(struct asn_type_selector_result_s *, struct asn_TYPE_descriptor_s *, void *);
+  struct asn_encoding_constraints_s encoding_constraints;
+  int (*default_value_cmp)(void *);
+  int (*default_value_set)(void **);
+  signed char *name;
+};
+
+struct ASN__PRIMITIVE_TYPE_s {
+  unsigned char *buf;
+  unsigned int size;
+};
+
+struct asn_INTEGER_enum_map_s {
+  int nat_value;
+  unsigned int enum_len;
+  signed char *enum_name;
+};
+
+struct asn_INTEGER_specifics_s {
+  struct asn_INTEGER_enum_map_s *value2enum;
+  unsigned int *enum2value;
+  int map_count;
+  int extension;
+  int strict_enumeration;
+  int field_width;
+  int field_unsigned;
+};
+
+union _2079 {
+  unsigned char *c_buf;
+  unsigned char *nc_buf;
+};
+
+struct e2v_key {
+  signed char *start;
+  signed char *stop;
+  struct asn_INTEGER_enum_map_s *vemap;
+  unsigned int *evmap;
+};
+
+extern unsigned int __compcert_va_int32(void *);
+extern unsigned long long __compcert_va_int64(void *);
+extern double __compcert_va_float64(void *);
+extern void *__compcert_va_composite(void *, unsigned int);
+extern long long __compcert_i64_dtos(double);
+extern unsigned long long __compcert_i64_dtou(double);
+extern double __compcert_i64_stod(long long);
+extern double __compcert_i64_utod(unsigned long long);
+extern float __compcert_i64_stof(long long);
+extern float __compcert_i64_utof(unsigned long long);
+extern long long __compcert_i64_sdiv(long long, long long);
+extern unsigned long long __compcert_i64_udiv(unsigned long long, unsigned long long);
+extern long long __compcert_i64_smod(long long, long long);
+extern unsigned long long __compcert_i64_umod(unsigned long long, unsigned long long);
+extern long long __compcert_i64_shl(long long, int);
+extern unsigned long long __compcert_i64_shr(unsigned long long, int);
+extern long long __compcert_i64_sar(long long, int);
+extern long long __compcert_i64_smulh(long long, long long);
+extern unsigned long long __compcert_i64_umulh(unsigned long long, unsigned long long);
+extern void __builtin_debug(int, ...);
+extern void *malloc(unsigned int);
+extern void *calloc(unsigned int, unsigned int);
+extern void *realloc(void *, unsigned int);
+extern void free(void *);
+extern void *bsearch(void *, void *, unsigned int, unsigned int, int (*)(void *, void *));
+extern int memcmp(void *, void *, unsigned int);
+extern int asn_get_few_bits(struct asn_bit_data_s *, int);
+extern int asn_get_many_bits(struct asn_bit_data_s *, unsigned char *, int, int);
+extern int asn_put_few_bits(struct asn_bit_outp_s *, unsigned int, int);
+extern int asn_put_many_bits(struct asn_bit_outp_s *, unsigned char *, int);
+extern int uper_get_length(struct asn_bit_data_s *, int, unsigned int, int *);
+extern int uper_get_constrained_whole_number(struct asn_bit_data_s *, unsigned int *, int);
+extern int per_long_range_rebase(int, int, int, unsigned int *);
+extern int per_long_range_unrebase(unsigned int, int, int, int *);
+extern int uper_put_constrained_whole_number_u(struct asn_bit_outp_s *, unsigned int, int);
+extern int uper_put_length(struct asn_bit_outp_s *, unsigned int, int *);
+extern int asn_generic_no_constraint(struct asn_TYPE_descriptor_s *, void *, void (*)(void *, struct asn_TYPE_descriptor_s *, void *, signed char *, ...), void *);
+extern int asn_generic_unknown_constraint(struct asn_TYPE_descriptor_s *, void *, void (*)(void *, struct asn_TYPE_descriptor_s *, void *, signed char *, ...), void *);
+extern long long asn_random_between(long long, long long);
+extern void oer_decode_primitive(struct asn_dec_rval_s *, struct asn_codec_ctx_s *, struct asn_TYPE_descriptor_s *, struct asn_oer_constraints_s *, void **, void *, unsigned int);
+extern void oer_encode_primitive(struct asn_enc_rval_s *, struct asn_TYPE_descriptor_s *, struct asn_oer_constraints_s *, void *, int (*)(void *, unsigned int, void *), void *);
+extern unsigned int asn_TYPE_outmost_tag(struct asn_TYPE_descriptor_s *, void *, int, unsigned int);
+extern void __assert_fail(signed char *, signed char *, unsigned int, signed char *);
+extern int asn__format_to_callback(int (*)(void *, unsigned int, void *), void *, signed char *, ...);
+extern void ASN__PRIMITIVE_TYPE_free(struct asn_TYPE_descriptor_s *, void *, int);
+extern void ber_decode_primitive(struct asn_dec_rval_s *, struct asn_codec_ctx_s *, struct asn_TYPE_descriptor_s *, void **, void *, unsigned int, int);
+extern void der_encode_primitive(struct asn_enc_rval_s *, struct asn_TYPE_descriptor_s *, void *, int, unsigned int, int (*)(void *, unsigned int, void *), void *);
+extern void xer_decode_primitive(struct asn_dec_rval_s *, struct asn_codec_ctx_s *, struct asn_TYPE_descriptor_s *, void **, unsigned int, signed char *, void *, unsigned int, int (*)(struct asn_TYPE_descriptor_s *, void *, void *, unsigned int));
+extern void INTEGER_decode_oer(struct asn_dec_rval_s *, struct asn_codec_ctx_s *, struct asn_TYPE_descriptor_s *, struct asn_oer_constraints_s *, void **, void *, unsigned int);
+extern void INTEGER_encode_oer(struct asn_enc_rval_s *, struct asn_TYPE_descriptor_s *, struct asn_oer_constraints_s *, void *, int (*)(void *, unsigned int, void *), void *);
+extern int *__errno_location(void);
+void INTEGER_encode_der(struct asn_enc_rval_s *, struct asn_TYPE_descriptor_s *, void *, int, unsigned int, int (*)(void *, unsigned int, void *), void *);
+int INTEGER__dump(struct asn_TYPE_descriptor_s *, struct ASN__PRIMITIVE_TYPE_s *, int (*)(void *, unsigned int, void *), void *, int);
+int INTEGER_print(struct asn_TYPE_descriptor_s *, void *, int, int (*)(void *, unsigned int, void *), void *);
+int INTEGER__compar_enum2value(void *, void *);
+struct asn_INTEGER_enum_map_s *INTEGER_map_enum2value(struct asn_INTEGER_specifics_s *, signed char *, signed char *);
+int INTEGER__compar_value2enum(void *, void *);
+struct asn_INTEGER_enum_map_s *INTEGER_map_value2enum(struct asn_INTEGER_specifics_s *, int);
+int INTEGER_st_prealloc(struct ASN__PRIMITIVE_TYPE_s *, int);
+int INTEGER__xer_body_decode(struct asn_TYPE_descriptor_s *, void *, void *, unsigned int);
+void INTEGER_decode_xer(struct asn_dec_rval_s *, struct asn_codec_ctx_s *, struct asn_TYPE_descriptor_s *, void **, signed char *, void *, unsigned int);
+void INTEGER_encode_xer(struct asn_enc_rval_s *, struct asn_TYPE_descriptor_s *, void *, int, int, int (*)(void *, unsigned int, void *), void *);
+void INTEGER_decode_uper(struct asn_dec_rval_s *, struct asn_codec_ctx_s *, struct asn_TYPE_descriptor_s *, struct asn_per_constraints_s *, void **, struct asn_bit_data_s *);
+void INTEGER_encode_uper(struct asn_enc_rval_s *, struct asn_TYPE_descriptor_s *, struct asn_per_constraints_s *, void *, struct asn_bit_outp_s *);
+long long asn__integer_convert(unsigned char *, unsigned char *);
+int asn_INTEGER2imax(struct ASN__PRIMITIVE_TYPE_s *, long long *);
+int asn_INTEGER2umax(struct ASN__PRIMITIVE_TYPE_s *, unsigned long long *);
+int asn_umax2INTEGER(struct ASN__PRIMITIVE_TYPE_s *, unsigned long long);
+int asn_imax2INTEGER(struct ASN__PRIMITIVE_TYPE_s *, long long);
+int asn_INTEGER2long(struct ASN__PRIMITIVE_TYPE_s *, int *);
+int asn_INTEGER2ulong(struct ASN__PRIMITIVE_TYPE_s *, unsigned int *);
+int asn_long2INTEGER(struct ASN__PRIMITIVE_TYPE_s *, int);
+int asn_ulong2INTEGER(struct ASN__PRIMITIVE_TYPE_s *, unsigned int);
+int asn_strtoimax_lim(signed char *, signed char **, long long *);
+int asn_strtoumax_lim(signed char *, signed char **, unsigned long long *);
+int asn_strtol_lim(signed char *, signed char **, int *);
+int asn_strtoul_lim(signed char *, signed char **, unsigned int *);
+int INTEGER_compare(struct asn_TYPE_descriptor_s *, void *, void *);
+void INTEGER_random_fill(struct asn_random_fill_result_s *, struct asn_TYPE_descriptor_s *, void **, struct asn_encoding_constraints_s *, unsigned int);
+signed char const __stringlit_10[12] = "Unreachable";
+
+signed char const __stringlit_6[17] = "0123456789ABCDEF";
+
+signed char const __stringlit_11[18] = "variants[18] == 0";
+
+signed char const __stringlit_1[8] = "INTEGER";
+
+signed char const __stringlit_4[6] = "<%s/>";
+
+signed char const __stringlit_2[5] = "%lld";
+
+signed char const __stringlit_3[5] = "%llu";
+
+signed char const __stringlit_5[10] = "%lld (%s)";
+
+signed char const __stringlit_7[9] = "<absent>";
+
+signed char const __stringlit_8[32] = "../../asn1c/skeletons/INTEGER.c";
+
+signed char const __stringlit_12[13] = "emap_len > 0";
+
+signed char const __stringlit_9[15] = "!\042Unreachable\042";
+
+unsigned int const asn_DEF_INTEGER_tags[1] = { 8, };
+
+struct asn_TYPE_operation_s asn_OP_INTEGER = { &ASN__PRIMITIVE_TYPE_free,
+  &INTEGER_print, &INTEGER_compare, &ber_decode_primitive,
+  &INTEGER_encode_der, &INTEGER_decode_xer, &INTEGER_encode_xer,
+  &INTEGER_decode_oer, &INTEGER_encode_oer, &INTEGER_decode_uper,
+  &INTEGER_encode_uper, &INTEGER_random_fill, 0, };
+
+struct asn_TYPE_descriptor_s asn_DEF_INTEGER = { &__stringlit_1,
+  &__stringlit_1, &asn_OP_INTEGER, &asn_DEF_INTEGER_tags, 1,
+  &asn_DEF_INTEGER_tags, 1, 0, 0, &asn_generic_no_constraint, 0, 0, 0, };
+
+void INTEGER_encode_der(struct asn_enc_rval_s *$_res, struct asn_TYPE_descriptor_s *$td, void *$sptr, int $tag_mode, unsigned int $tag, int (*$cb)(void *, unsigned int, void *), void *$app_key)
+{
+  struct asn_enc_rval_s rval;
+  struct ASN__PRIMITIVE_TYPE_s effective_integer;
+  union _2079 unconst;
+  struct asn_enc_rval_s _res__1;
+  register struct ASN__PRIMITIVE_TYPE_s *$st;
+  register unsigned char *$buf;
+  register unsigned char *$end1;
+  register int $shift;
+  register unsigned int $349;
+  register unsigned char $348;
+  register unsigned char $347;
+  register unsigned char $346;
+  register unsigned char *$345;
+  register unsigned char *$344;
+  register unsigned char *$343;
+  register unsigned int $342;
+  register unsigned char *$341;
+  register void *$340;
+  $st = (struct ASN__PRIMITIVE_TYPE_s *) $sptr;
+  for (; 1; ({ break; })) {
+    /*skip*/;
+  }
+  $341 = (*$st).buf;
+  if ($341) {
+    $buf = (*$st).buf;
+    $349 = (*$st).size;
+    $end1 = $buf + $349 - 1;
+    for (; 1; $buf = $buf + 1) {
+      if (! ($buf < $end1)) {
+        break;
+      }
+      $346 = *$buf;
+      switch ($346) {
+        case 0:
+          $348 = *($buf + 1);
+          if (($348 & 128) == 0) {
+            continue;
+          }
+          break;
+        case 255:
+          $347 = *($buf + 1);
+          if ($347 & 128) {
+            continue;
+          }
+          break;
+        
+      }
+      break;
+    }
+    $345 = (*$st).buf;
+    $shift = $buf - $345;
+    if ($shift) {
+      $344 = (*$st).buf;
+      unconst.c_buf = $344;
+      $343 = unconst.nc_buf;
+      effective_integer.buf = $343 + $shift;
+      $342 = (*$st).size;
+      effective_integer.size = $342 - $shift;
+      $st = &effective_integer;
+    }
+  }
+  der_encode_primitive(&_res__1, $td, $st, $tag_mode, $tag, $cb, $app_key);
+  rval = _res__1;
+  $340 = rval.structure_ptr;
+  if ($340 == &effective_integer) {
+    rval.structure_ptr = $sptr;
+  }
+  *$_res = rval;
+  return;
+}
+
+int INTEGER__dump(struct asn_TYPE_descriptor_s *$td, struct ASN__PRIMITIVE_TYPE_s *$st, int (*$cb)(void *, unsigned int, void *), void *$app_key, int $plainOrXER)
+{
+  signed char scratch[32];
+  long long value;
+  register struct asn_INTEGER_specifics_s *$specs;
+  register unsigned char *$buf;
+  register unsigned char *$buf_end;
+  register int $wrote;
+  register signed char *$p;
+  register int $ret;
+  register struct asn_INTEGER_enum_map_s *$el;
+  register signed char *$h2c;
+  register int $363;
+  register int $362;
+  register signed char *$361;
+  register signed char *$360;
+  register signed char *$359;
+  register int $358;
+  register int $357;
+  register int $356;
+  register int *$355;
+  register int $354;
+  register int $353;
+  register int $352;
+  register signed char *$351;
+  register int $350;
+  register int *$349;
+  register int $348;
+  register int $347;
+  register struct asn_INTEGER_enum_map_s *$346;
+  register void *$345;
+  register int $344;
+  register int $343;
+  register int $342;
+  register int $341;
+  register int $340;
+  register void *$381;
+  register unsigned int $380;
+  register unsigned char *$379;
+  register int $378;
+  register long long $377;
+  register int $376;
+  register long long $375;
+  register signed char *$374;
+  register long long $373;
+  register signed char *$372;
+  register int $371;
+  register int $370;
+  register long long $369;
+  register int $368;
+  register signed char $367;
+  register unsigned char $366;
+  register signed char $365;
+  register unsigned char $364;
+  $381 = (*$td).specifics;
+  $specs = (struct asn_INTEGER_specifics_s *) $381;
+  $buf = (*$st).buf;
+  $379 = (*$st).buf;
+  $380 = (*$st).size;
+  $buf_end = $379 + $380;
+  $wrote = 0;
+  if ($specs) {
+    $378 = (*$specs).field_unsigned;
+    $342 = (_Bool) $378;
+  } else {
+    $342 = 0;
+  }
+  if ($342) {
+    $340 = asn_INTEGER2umax($st, (unsigned long long *) &value);
+    $ret = $340;
+  } else {
+    $341 = asn_INTEGER2imax($st, &value);
+    $ret = $341;
+  }
+  if ($ret == 0) {
+    $377 = value;
+    if ($377 >= 0) {
+      $343 = 1;
+    } else {
+      $343 = (_Bool) !$specs;
+    }
+    if ($343) {
+      $344 = 1;
+    } else {
+      $376 = (*$specs).field_unsigned;
+      $344 = (_Bool) !$376;
+    }
+    if ($344) {
+      $375 = value;
+      $346 = INTEGER_map_value2enum($specs, $375);
+      $345 = (void *) $346;
+    } else {
+      $345 = (void *) (void *) 0;
+    }
+    $el = $345;
+    if ($el) {
+      if ($plainOrXER == 0) {
+        $373 = value;
+        $374 = (*$el).enum_name;
+        $347 =
+          asn__format_to_callback
+          ($cb, $app_key, __stringlit_5, $373, $374);
+        return $347;
+      } else {
+        $372 = (*$el).enum_name;
+        $348 = asn__format_to_callback($cb, $app_key, __stringlit_4, $372);
+        return $348;
+      }
+    } else {
+      if ($plainOrXER) {
+        $353 = (_Bool) $specs;
+      } else {
+        $353 = 0;
+      }
+      if ($353) {
+        $371 = (*$specs).strict_enumeration;
+        $354 = (_Bool) $371;
+      } else {
+        $354 = 0;
+      }
+      if ($354) {
+        for (; 1; ({ break; })) {
+          /*skip*/;
+        }
+        $349 = __errno_location();
+        *$349 = 1;
+        return -1;
+      } else {
+        if ($specs) {
+          $370 = (*$specs).field_unsigned;
+          $350 = (_Bool) $370;
+        } else {
+          $350 = 0;
+        }
+        if ($350) {
+          $351 = (signed char *) __stringlit_3;
+        } else {
+          $351 = (signed char *) __stringlit_2;
+        }
+        $369 = value;
+        $352 = asn__format_to_callback($cb, $app_key, $351, $369);
+        return $352;
+      }
+    }
+  } else {
+    if ($plainOrXER) {
+      $356 = (_Bool) $specs;
+    } else {
+      $356 = 0;
+    }
+    if ($356) {
+      $368 = (*$specs).strict_enumeration;
+      $357 = (_Bool) $368;
+    } else {
+      $357 = 0;
+    }
+    if ($357) {
+      for (; 1; ({ break; })) {
+        /*skip*/;
+      }
+      $355 = __errno_location();
+      *$355 = 1;
+      return -1;
+    }
+  }
+  $p = scratch;
+  for (; 1; $buf = $buf + 1) {
+    if (! ($buf < $buf_end)) {
+      break;
+    }
+    $h2c = __stringlit_6;
+    if ($p - scratch >= (int) (sizeof(signed char [32]) - 4)) {
+      $358 = $cb(scratch, $p - scratch, $app_key);
+      if ($358 < 0) {
+        return -1;
+      }
+      $wrote = $wrote + ($p - scratch);
+      $p = scratch;
+    }
+    $359 = $p;
+    $p = $359 + 1;
+    $366 = *$buf;
+    $367 = *($h2c + ($366 >> 4));
+    *$359 = $367;
+    $360 = $p;
+    $p = $360 + 1;
+    $364 = *$buf;
+    $365 = *($h2c + ($364 & 15));
+    *$360 = $365;
+    $361 = $p;
+    $p = $361 + 1;
+    *$361 = 58;
+  }
+  if ($p != scratch) {
+    $p = $p - 1;
+  }
+  $wrote = $wrote + ($p - scratch);
+  $362 = $cb(scratch, $p - scratch, $app_key);
+  if ($362 < 0) {
+    $363 = (int) -1;
+  } else {
+    $363 = (int) $wrote;
+  }
+  return $363;
+}
+
+int INTEGER_print(struct asn_TYPE_descriptor_s *$td, void *$sptr, int $ilevel, int (*$cb)(void *, unsigned int, void *), void *$app_key)
+{
+  register struct ASN__PRIMITIVE_TYPE_s *$st;
+  register int $ret;
+  register int $343;
+  register int $342;
+  register int $341;
+  register int $340;
+  register unsigned char *$344;
+  $st = (struct ASN__PRIMITIVE_TYPE_s *) $sptr;
+  if (!$st) {
+    $342 = 1;
+  } else {
+    $344 = (*$st).buf;
+    $342 = (_Bool) !$344;
+  }
+  if ($342) {
+    $340 = $cb(__stringlit_7, 8, $app_key);
+    $ret = $340;
+  } else {
+    $341 = INTEGER__dump($td, $st, $cb, $app_key, 0);
+    $ret = $341;
+  }
+  if ($ret < 0) {
+    $343 = (int) -1;
+  } else {
+    $343 = (int) 0;
+  }
+  return $343;
+}
+
+int INTEGER__compar_enum2value(void *$kp, void *$am)
+{
+  register struct e2v_key *$key;
+  register struct asn_INTEGER_enum_map_s *$el;
+  register signed char *$ptr;
+  register signed char *$end;
+  register signed char *$name;
+  register int $341;
+  register int $340;
+  register unsigned int $351;
+  register struct asn_INTEGER_enum_map_s *$350;
+  register unsigned int *$349;
+  register struct asn_INTEGER_enum_map_s *$348;
+  register signed char $347;
+  register signed char $346;
+  register signed char $345;
+  register unsigned char $344;
+  register unsigned char $343;
+  register signed char $342;
+  $key = (struct e2v_key *) $kp;
+  $el = (struct asn_INTEGER_enum_map_s *) $am;
+  $348 = (*$key).vemap;
+  $349 = (*$key).evmap;
+  $350 = (*$key).vemap;
+  $351 = *($349 + ($el - $350));
+  $el = $348 + $351;
+  $ptr = (*$key).start;
+  $end = (*$key).stop;
+  $name = (*$el).enum_name;
+  for (; 1; $ptr = $ptr + 1, $name = $name + 1) {
+    if (! ($ptr < $end)) {
+      break;
+    }
+    $345 = *$ptr;
+    $346 = *$name;
+    if ($345 != $346) {
+      $340 = 1;
+    } else {
+      $347 = *$name;
+      $340 = (_Bool) !$347;
+    }
+    if ($340) {
+      $343 = *((unsigned char *) $ptr);
+      $344 = *((unsigned char *) $name);
+      return $343 - $344;
+    }
+  }
+  $342 = *($name + 0);
+  if ($342) {
+    $341 = (int) -1;
+  } else {
+    $341 = (int) 0;
+  }
+  return $341;
+}
+
+struct asn_INTEGER_enum_map_s *INTEGER_map_enum2value(struct asn_INTEGER_specifics_s *$specs, signed char *$lstart, signed char *$lstop)
+{
+  struct e2v_key key;
+  register struct asn_INTEGER_enum_map_s *$el_found;
+  register int $count;
+  register signed char *$lp;
+  register void *$341;
+  register int $340;
+  register int $350;
+  register signed char $349;
+  register struct asn_INTEGER_enum_map_s *$348;
+  register unsigned int *$347;
+  register struct asn_INTEGER_enum_map_s *$346;
+  register unsigned int $345;
+  register struct asn_INTEGER_enum_map_s *$344;
+  register unsigned int *$343;
+  register struct asn_INTEGER_enum_map_s *$342;
+  if ($specs) {
+    $350 = (*$specs).map_count;
+    $340 = (int) $350;
+  } else {
+    $340 = (int) 0;
+  }
+  $count = $340;
+  if (!$count) {
+    return (void *) 0;
+  }
+  $lstart = $lstart + 1;
+  $lp = $lstart;
+  for (; 1; $lp = $lp + 1) {
+    if (! ($lp < $lstop)) {
+      break;
+    }
+    $349 = *$lp;
+    switch ($349) {
+      case 9:
+      case 10:
+      case 11:
+      case 12:
+      case 13:
+      case 32:
+      case 47:
+      case 62:
+        break;
+      default:
+        continue;
+      
+    }
+    break;
+  }
+  if ($lp == $lstop) {
+    return (void *) 0;
+  }
+  $lstop = $lp;
+  key.start = $lstart;
+  key.stop = $lstop;
+  $348 = (*$specs).value2enum;
+  key.vemap = $348;
+  $347 = (*$specs).enum2value;
+  key.evmap = $347;
+  $346 = (*$specs).value2enum;
+  $341 =
+    bsearch
+    (&key, $346, $count, sizeof(struct asn_INTEGER_enum_map_s),
+     INTEGER__compar_enum2value);
+  $el_found = (struct asn_INTEGER_enum_map_s *) $341;
+  if ($el_found) {
+    $342 = key.vemap;
+    $343 = key.evmap;
+    $344 = key.vemap;
+    $345 = *($343 + ($el_found - $344));
+    $el_found = $342 + $345;
+  }
+  return $el_found;
+}
+
+int INTEGER__compar_value2enum(void *$kp, void *$am)
+{
+  register int $a;
+  register struct asn_INTEGER_enum_map_s *$el;
+  register int $b;
+  $a = *((int *) $kp);
+  $el = (struct asn_INTEGER_enum_map_s *) $am;
+  $b = (*$el).nat_value;
+  if ($a < $b) {
+    return -1;
+  } else {
+    if ($a == $b) {
+      return 0;
+    } else {
+      return 1;
+    }
+  }
+}
+
+struct asn_INTEGER_enum_map_s *INTEGER_map_value2enum(struct asn_INTEGER_specifics_s *$specs, int $value)
+{
+  int value;
+  register int $count;
+  register void *$341;
+  register int $340;
+  register int $343;
+  register struct asn_INTEGER_enum_map_s *$342;
+  value = $value;
+  if ($specs) {
+    $343 = (*$specs).map_count;
+    $340 = (int) $343;
+  } else {
+    $340 = (int) 0;
+  }
+  $count = $340;
+  if (!$count) {
+    return 0;
+  }
+  $342 = (*$specs).value2enum;
+  $341 =
+    bsearch
+    (&value, $342, $count, sizeof(struct asn_INTEGER_enum_map_s),
+     INTEGER__compar_value2enum);
+  return (struct asn_INTEGER_enum_map_s *) $341;
+}
+
+int INTEGER_st_prealloc(struct ASN__PRIMITIVE_TYPE_s *$st, int $min_size)
+{
+  register void *$p;
+  register void *$b;
+  register void *$340;
+  $340 = malloc($min_size + 1);
+  $p = $340;
+  if ($p) {
+    $b = (*$st).buf;
+    (*$st).size = 0;
+    (*$st).buf = $p;
+    free($b);
+    return 0;
+  } else {
+    return -1;
+  }
+}
+
+int INTEGER__xer_body_decode(struct asn_TYPE_descriptor_s *$td, void *$sptr, void *$chunk_buf, unsigned int $chunk_size)
+{
+  long long dec_value;
+  signed char *dec_value_end;
+  register struct ASN__PRIMITIVE_TYPE_s *$st;
+  register long long $hex_value;
+  register signed char *$lp;
+  register signed char *$lstart;
+  register signed char *$lstop;
+  register int $state;
+  register signed char *$dec_value_start;
+  register int $lv;
+  register struct asn_INTEGER_enum_map_s *$el;
+  register int $348;
+  register int $347;
+  register int $346;
+  register unsigned int $345;
+  register int $344;
+  register int $343;
+  register struct asn_INTEGER_enum_map_s *$342;
+  register unsigned int $341;
+  register int $340;
+  register unsigned char *$357;
+  register void *$356;
+  register int $355;
+  register unsigned char *$354;
+  register long long $353;
+  register long long $352;
+  register unsigned int $351;
+  register unsigned char *$350;
+  register long long $349;
+  $st = (struct ASN__PRIMITIVE_TYPE_s *) $sptr;
+  $hex_value = (long long) 0;
+  $lstart = (signed char *) $chunk_buf;
+  $lstop = $lstart + $chunk_size;
+  $state = 0;
+  $dec_value_start = 0;
+  dec_value_end = 0;
+  if ($chunk_size) {
+    for (; 1; ({ break; })) {
+      /*skip*/;
+    }
+  }
+  $340 = INTEGER_st_prealloc($st, $chunk_size / 3 + 1);
+  if ($340) {
+    return 0;
+  }
+  $lp = $lstart;
+  for (; 1; $lp = $lp + 1) {
+    if (! ($lp < $lstop)) {
+      break;
+    }
+    $lv = *$lp;
+    switch ($lv) {
+      case 9:
+      case 10:
+      case 13:
+      case 32:
+        switch ($state) {
+          case 0:
+          case 4:
+          case 7:
+          case 1:
+            continue;
+          case 3:
+            dec_value_end = $lp;
+            $state = 4;
+            continue;
+          case 8:
+            $state = 7;
+            continue;
+          default:
+            break;
+          
+        }
+        break;
+      case 45:
+        if ($state == 0) {
+          dec_value = 0;
+          $dec_value_start = $lp;
+          $state = 2;
+          continue;
+        }
+        break;
+      case 43:
+        if ($state == 0) {
+          dec_value = 0;
+          $dec_value_start = $lp;
+          $state = 2;
+          continue;
+        }
+        break;
+      case 48:
+      case 49:
+      case 50:
+      case 51:
+      case 52:
+      case 53:
+      case 54:
+      case 55:
+      case 56:
+      case 57:
+        switch ($state) {
+          case 3:
+            continue;
+          case 1:
+          case 5:
+            $hex_value = (long long) ($lv - 48 << 4);
+            $state = 6;
+            continue;
+          case 6:
+            $hex_value = $hex_value + ($lv - 48);
+            $state = 8;
+            $341 = (*$st).size;
+            (*$st).size = $341 + 1;
+            $357 = (*$st).buf;
+            *($357 + $341) = (unsigned char) $hex_value;
+            continue;
+          case 8:
+            return 2;
+          case 0:
+            dec_value = 0;
+            $dec_value_start = $lp;
+          case 2:
+            $state = 3;
+            continue;
+          default:
+            break;
+          
+        }
+        break;
+      case 60:
+        if ($state == 0) {
+          $356 = (*$td).specifics;
+          $342 =
+            INTEGER_map_enum2value
+            ((struct asn_INTEGER_specifics_s *) $356, $lstart, $lstop);
+          $el = $342;
+          if ($el) {
+            for (; 1; ({ break; })) {
+              /*skip*/;
+            }
+            $355 = (*$el).nat_value;
+            dec_value = $355;
+            $state = 9;
+            $lp = $lstop - 1;
+            continue;
+          }
+          for (; 1; ({ break; })) {
+            /*skip*/;
+          }
+        }
+        return 2;
+      case 58:
+        if ($state == 8) {
+          $state = 5;
+          continue;
+        } else {
+          if ($state == 3) {
+            for (; 1; ({ break; })) {
+              /*skip*/;
+            }
+            $state = 1;
+            $dec_value_start = 0;
+            $lp = $lstart - 1;
+            continue;
+          } else {
+            for (; 1; ({ break; })) {
+              /*skip*/;
+            }
+            break;
+          }
+        }
+      case 65:
+      case 66:
+      case 67:
+      case 68:
+      case 69:
+      case 70:
+      case 97:
+      case 98:
+      case 99:
+      case 100:
+      case 101:
+      case 102:
+        switch ($state) {
+          case 1:
+          case 0:
+          case 5:
+            if ($lv < 97) {
+              $343 = (int) 65;
+            } else {
+              $343 = (int) 97;
+            }
+            $hex_value = (long long) ($lv - $343);
+            $hex_value = $hex_value + 10;
+            $hex_value = $hex_value << 4;
+            $state = 6;
+            continue;
+          case 6:
+            if ($lv < 97) {
+              $344 = (int) 65;
+            } else {
+              $344 = (int) 97;
+            }
+            $hex_value = $hex_value + ($lv - $344);
+            $hex_value = $hex_value + 10;
+            $345 = (*$st).size;
+            (*$st).size = $345 + 1;
+            $354 = (*$st).buf;
+            *($354 + $345) = (unsigned char) $hex_value;
+            $state = 8;
+            continue;
+          case 3:
+            for (; 1; ({ break; })) {
+              /*skip*/;
+            }
+            $state = 1;
+            $dec_value_start = 0;
+            $lp = $lstart - 1;
+            continue;
+          default:
+            break;
+          
+        }
+        break;
+      
+    }
+    for (; 1; ({ break; })) {
+      /*skip*/;
+    }
+    $state = 10;
+    break;
+  }
+  switch ($state) {
+    case 9:
+      break;
+    case 3:
+      dec_value_end = $lstop;
+    case 4:
+      $346 = asn_strtoimax_lim($dec_value_start, &dec_value_end, &dec_value);
+      switch ($346) {
+        case 0:
+          $352 = dec_value;
+          if ($352 >= -2147483647 - 1) {
+            $353 = dec_value;
+            $347 = (_Bool) ($353 <= 2147483647);
+          } else {
+            $347 = 0;
+          }
+          if ($347) {
+            break;
+          } else {
+            for (; 1; ({ break; })) {
+              /*skip*/;
+            }
+          }
+        case 4294967293:
+          for (; 1; ({ break; })) {
+            /*skip*/;
+          }
+          return 1;
+        case 4294967294:
+        case 4294967295:
+        case 1:
+          return 2;
+        
+      }
+      break;
+    case 8:
+    case 7:
+      $350 = (*$st).buf;
+      $351 = (*$st).size;
+      *($350 + $351) = 0;
+      return 4;
+    case 5:
+    case 6:
+    case 1:
+      return 2;
+    case 0:
+      return 3;
+    case 2:
+    case 10:
+      for (; 1; ({ break; })) {
+        /*skip*/;
+      }
+      return 2;
+    
+  }
+  $349 = dec_value;
+  $348 = asn_imax2INTEGER($st, $349);
+  if ($348) {
+    for (; 1; ({ break; })) {
+      /*skip*/;
+    }
+    return 0;
+  }
+  return 4;
+}
+
+void INTEGER_decode_xer(struct asn_dec_rval_s *$_res, struct asn_codec_ctx_s *$opt_codec_ctx, struct asn_TYPE_descriptor_s *$td, void **$sptr, signed char *$opt_mname, void *$buf_ptr, unsigned int $size)
+{
+  struct asn_dec_rval_s _res__1;
+  xer_decode_primitive
+    (&_res__1, $opt_codec_ctx, $td, $sptr,
+     sizeof(struct ASN__PRIMITIVE_TYPE_s), $opt_mname, $buf_ptr, $size,
+     INTEGER__xer_body_decode);
+  *$_res = _res__1;
+  return;
+}
+
+void INTEGER_encode_xer(struct asn_enc_rval_s *$_res, struct asn_TYPE_descriptor_s *$td, void *$sptr, int $ilevel, int $flags, int (*$cb)(void *, unsigned int, void *), void *$app_key)
+{
+  struct asn_enc_rval_s er;
+  struct asn_enc_rval_s tmp_error;
+  struct asn_enc_rval_s tmp_error__1;
+  register struct ASN__PRIMITIVE_TYPE_s *$st;
+  register int $341;
+  register int $340;
+  register unsigned char *$343;
+  register int $342;
+  $st = (struct ASN__PRIMITIVE_TYPE_s *) $sptr;
+  if (!$st) {
+    $340 = 1;
+  } else {
+    $343 = (*$st).buf;
+    $340 = (_Bool) !$343;
+  }
+  if ($340) {
+    for (; 1; ({ break; })) {
+      tmp_error.encoded = -1;
+      tmp_error.failed_type = $td;
+      tmp_error.structure_ptr = $sptr;
+      for (; 1; ({ break; })) {
+        /*skip*/;
+      }
+      *$_res = tmp_error;
+      return;
+    }
+  }
+  $341 = INTEGER__dump($td, $st, $cb, $app_key, 1);
+  er.encoded = $341;
+  $342 = er.encoded;
+  if ($342 < 0) {
+    for (; 1; ({ break; })) {
+      tmp_error__1.encoded = -1;
+      tmp_error__1.failed_type = $td;
+      tmp_error__1.structure_ptr = $sptr;
+      for (; 1; ({ break; })) {
+        /*skip*/;
+      }
+      *$_res = tmp_error__1;
+      return;
+    }
+  }
+  for (; 1; ({ break; })) {
+    er.structure_ptr = 0;
+    er.failed_type = 0;
+    *$_res = er;
+    return;
+  }
+}
+
+void INTEGER_decode_uper(struct asn_dec_rval_s *$_res, struct asn_codec_ctx_s *$opt_codec_ctx, struct asn_TYPE_descriptor_s *$td, struct asn_per_constraints_s *$constraints, void **$sptr, struct asn_bit_data_s *$pd)
+{
+  struct asn_dec_rval_s rval;
+  int repeat;
+  struct asn_dec_rval_s tmp_error;
+  struct asn_dec_rval_s tmp_error__1;
+  struct asn_dec_rval_s tmp_error__2;
+  struct asn_dec_rval_s tmp_error__3;
+  struct asn_dec_rval_s tmp_error__4;
+  unsigned int uvalue;
+  struct asn_dec_rval_s tmp_error__5;
+  struct asn_dec_rval_s tmp_error__6;
+  unsigned int uvalue__1;
+  int svalue;
+  struct asn_dec_rval_s tmp_error__7;
+  struct asn_dec_rval_s tmp_error__8;
+  struct asn_dec_rval_s tmp_error__9;
+  struct asn_dec_rval_s tmp_error__10;
+  struct asn_dec_rval_s tmp_error__11;
+  int value;
+  struct asn_dec_rval_s tmp_error__12;
+  struct asn_dec_rval_s tmp_error__13;
+  register struct asn_INTEGER_specifics_s *$specs;
+  register struct ASN__PRIMITIVE_TYPE_s *$st;
+  register struct asn_per_constraint_s *$ct;
+  register int $inext;
+  register unsigned int $size;
+  register int $len;
+  register void *$p;
+  register int $ret;
+  register int $361;
+  register int $360;
+  register int $359;
+  register int $358;
+  register void *$357;
+  register int $356;
+  register int $355;
+  register int $354;
+  register int $353;
+  register int $352;
+  register int $351;
+  register int $350;
+  register int $349;
+  register int $348;
+  register int $347;
+  register void *$346;
+  register void *$345;
+  register int $344;
+  register int $343;
+  register void *$342;
+  register void *$341;
+  register void *$340;
+  register void *$395;
+  register void *$394;
+  register int $393;
+  register unsigned char *$392;
+  register unsigned char *$391;
+  register int $390;
+  register int $389;
+  register int $388;
+  register unsigned char *$387;
+  register int $386;
+  register int $385;
+  register int $384;
+  register int $383;
+  register int $382;
+  register int $381;
+  register unsigned int $380;
+  register unsigned int $379;
+  register int $378;
+  register int $377;
+  register int $376;
+  register unsigned int $375;
+  register int $374;
+  register int $373;
+  register unsigned int $372;
+  register unsigned char *$371;
+  register unsigned int $370;
+  register unsigned char *$369;
+  register unsigned int $368;
+  register int $367;
+  register unsigned int $366;
+  register unsigned char *$365;
+  register int $364;
+  register int $363;
+  register int $362;
+  $395 = (*$td).specifics;
+  $specs = (struct asn_INTEGER_specifics_s *) $395;
+  rval.code = 0;
+  rval.consumed = 0;
+  $394 = *$sptr;
+  $st = (struct ASN__PRIMITIVE_TYPE_s *) $394;
+  if (!$st) {
+    $340 = calloc(1, sizeof(struct ASN__PRIMITIVE_TYPE_s));
+    $341 = (void *) $340;
+    *$sptr = $341;
+    $st = (struct ASN__PRIMITIVE_TYPE_s *) $341;
+    if (!$st) {
+      for (; 1; ({ break; })) {
+        tmp_error.code = 2;
+        tmp_error.consumed = 0;
+        for (; 1; ({ break; })) {
+          /*skip*/;
+        }
+        *$_res = tmp_error;
+        return;
+      }
+    }
+  }
+  if (!$constraints) {
+    $constraints = (*$td).encoding_constraints.per_constraints;
+  }
+  if ($constraints) {
+    $342 = (void *) &(*$constraints).value;
+  } else {
+    $342 = (void *) (void *) 0;
+  }
+  $ct = $342;
+  if ($ct) {
+    $393 = (*$ct).flags;
+    $344 = (_Bool) ($393 & 4);
+  } else {
+    $344 = 0;
+  }
+  if ($344) {
+    $343 = asn_get_few_bits($pd, 1);
+    $inext = $343;
+    if ($inext < 0) {
+      for (; 1; ({ break; })) {
+        tmp_error__1.code = 1;
+        tmp_error__1.consumed = 0;
+        *$_res = tmp_error__1;
+        return;
+      }
+    }
+    if ($inext) {
+      $ct = 0;
+    }
+  }
+  $392 = (*$st).buf;
+  free($392);
+  (*$st).buf = 0;
+  (*$st).size = 0;
+  if ($ct) {
+    $386 = (*$ct).flags;
+    if ($386 & 1) {
+      $345 = calloc(1, 2);
+      (*$st).buf = (unsigned char *) $345;
+      $391 = (*$st).buf;
+      if (!$391) {
+        for (; 1; ({ break; })) {
+          tmp_error__2.code = 2;
+          tmp_error__2.consumed = 0;
+          for (; 1; ({ break; })) {
+            /*skip*/;
+          }
+          *$_res = tmp_error__2;
+          return;
+        }
+      }
+      (*$st).size = 1;
+    } else {
+      $389 = (*$ct).flags;
+      if ($389 & 2) {
+        $390 = (*$ct).range_bits;
+        $347 = (_Bool) ($390 >= 0);
+      } else {
+        $347 = 0;
+      }
+      if ($347) {
+        $388 = (*$ct).range_bits;
+        $size = $388 + 7 >> 3;
+        $346 = malloc(1 + $size + 1);
+        (*$st).buf = (unsigned char *) $346;
+        $387 = (*$st).buf;
+        if (!$387) {
+          for (; 1; ({ break; })) {
+            tmp_error__3.code = 2;
+            tmp_error__3.consumed = 0;
+            for (; 1; ({ break; })) {
+              /*skip*/;
+            }
+            *$_res = tmp_error__3;
+            return;
+          }
+        }
+        (*$st).size = $size;
+      }
+    }
+  }
+  if ($ct) {
+    $385 = (*$ct).flags;
+    $355 = (_Bool) ($385 != 0);
+  } else {
+    $355 = 0;
+  }
+  if ($355) {
+    for (; 1; ({ break; })) {
+      /*skip*/;
+    }
+    $373 = (*$ct).range_bits;
+    if ($373 >= 0) {
+      $384 = (*$ct).range_bits;
+      if ((unsigned int) $384 > 8 * sizeof(unsigned int)) {
+        for (; 1; ({ break; })) {
+          tmp_error__4.code = 2;
+          tmp_error__4.consumed = 0;
+          for (; 1; ({ break; })) {
+            /*skip*/;
+          }
+          *$_res = tmp_error__4;
+          return;
+        }
+      }
+      if ($specs) {
+        $383 = (*$specs).field_unsigned;
+        $354 = (_Bool) $383;
+      } else {
+        $354 = 0;
+      }
+      if ($354) {
+        uvalue = 0;
+        $382 = (*$ct).range_bits;
+        $348 = uper_get_constrained_whole_number($pd, &uvalue, $382);
+        if ($348) {
+          for (; 1; ({ break; })) {
+            tmp_error__5.code = 1;
+            tmp_error__5.consumed = 0;
+            *$_res = tmp_error__5;
+            return;
+          }
+        }
+        for (; 1; ({ break; })) {
+          /*skip*/;
+        }
+        $380 = uvalue;
+        $381 = (*$ct).lower_bound;
+        uvalue = $380 + $381;
+        $379 = uvalue;
+        $349 = asn_ulong2INTEGER($st, $379);
+        if ($349) {
+          for (; 1; ({ break; })) {
+            tmp_error__6.code = 2;
+            tmp_error__6.consumed = 0;
+            for (; 1; ({ break; })) {
+              /*skip*/;
+            }
+            *$_res = tmp_error__6;
+            return;
+          }
+        }
+      } else {
+        uvalue__1 = 0;
+        $378 = (*$ct).range_bits;
+        $350 = uper_get_constrained_whole_number($pd, &uvalue__1, $378);
+        if ($350) {
+          for (; 1; ({ break; })) {
+            tmp_error__7.code = 1;
+            tmp_error__7.consumed = 0;
+            *$_res = tmp_error__7;
+            return;
+          }
+        }
+        for (; 1; ({ break; })) {
+          /*skip*/;
+        }
+        $375 = uvalue__1;
+        $376 = (*$ct).lower_bound;
+        $377 = (*$ct).upper_bound;
+        $351 = per_long_range_unrebase($375, $376, $377, &svalue);
+        if ($351) {
+          $352 = 1;
+        } else {
+          $374 = svalue;
+          $353 = asn_long2INTEGER($st, $374);
+          $352 = (_Bool) $353;
+        }
+        if ($352) {
+          for (; 1; ({ break; })) {
+            tmp_error__8.code = 2;
+            tmp_error__8.consumed = 0;
+            for (; 1; ({ break; })) {
+              /*skip*/;
+            }
+            *$_res = tmp_error__8;
+            return;
+          }
+        }
+      }
+      *$_res = rval;
+      return;
+    }
+  } else {
+    for (; 1; ({ break; })) {
+      /*skip*/;
+    }
+  }
+  for (; 1; $367 = repeat, ({ if (! $367) {
+                                break;
+                              } })) {
+    $len = 0;
+    $p = (void *) 0;
+    $ret = 0;
+    $356 = uper_get_length($pd, -1, 0, &repeat);
+    $len = $356;
+    if ($len < 0) {
+      for (; 1; ({ break; })) {
+        tmp_error__9.code = 1;
+        tmp_error__9.consumed = 0;
+        *$_res = tmp_error__9;
+        return;
+      }
+    }
+    $371 = (*$st).buf;
+    $372 = (*$st).size;
+    $357 = realloc($371, $372 + $len + 1);
+    $p = $357;
+    if (!$p) {
+      for (; 1; ({ break; })) {
+        tmp_error__10.code = 2;
+        tmp_error__10.consumed = 0;
+        for (; 1; ({ break; })) {
+          /*skip*/;
+        }
+        *$_res = tmp_error__10;
+        return;
+      }
+    }
+    (*$st).buf = (unsigned char *) $p;
+    $369 = (*$st).buf;
+    $370 = (*$st).size;
+    $358 = asn_get_many_bits($pd, $369 + $370, 0, 8 * $len);
+    $ret = $358;
+    if ($ret < 0) {
+      for (; 1; ({ break; })) {
+        tmp_error__11.code = 1;
+        tmp_error__11.consumed = 0;
+        *$_res = tmp_error__11;
+        return;
+      }
+    }
+    $368 = (*$st).size;
+    (*$st).size = $368 + $len;
+  }
+  $365 = (*$st).buf;
+  $366 = (*$st).size;
+  *($365 + $366) = 0;
+  if ($ct) {
+    $364 = (*$ct).lower_bound;
+    $361 = (_Bool) $364;
+  } else {
+    $361 = 0;
+  }
+  if ($361) {
+    value = 0;
+    $359 = asn_INTEGER2long($st, &value);
+    if ($359) {
+      for (; 1; ({ break; })) {
+        tmp_error__12.code = 2;
+        tmp_error__12.consumed = 0;
+        for (; 1; ({ break; })) {
+          /*skip*/;
+        }
+        *$_res = tmp_error__12;
+        return;
+      }
+    }
+    $362 = value;
+    $363 = (*$ct).lower_bound;
+    $360 = asn_imax2INTEGER($st, $362 + $363);
+    if ($360) {
+      for (; 1; ({ break; })) {
+        tmp_error__13.code = 2;
+        tmp_error__13.consumed = 0;
+        for (; 1; ({ break; })) {
+          /*skip*/;
+        }
+        *$_res = tmp_error__13;
+        return;
+      }
+    }
+  }
+  *$_res = rval;
+  return;
+}
+
+void INTEGER_encode_uper(struct asn_enc_rval_s *$_res, struct asn_TYPE_descriptor_s *$td, struct asn_per_constraints_s *$constraints, void *$sptr, struct asn_bit_outp_s *$po)
+{
+  struct asn_enc_rval_s er;
+  int value;
+  struct asn_enc_rval_s tmp_error;
+  unsigned int uval;
+  struct asn_enc_rval_s tmp_error__1;
+  struct asn_enc_rval_s tmp_error__2;
+  struct asn_enc_rval_s tmp_error__3;
+  struct asn_enc_rval_s tmp_error__4;
+  unsigned int v;
+  struct asn_enc_rval_s tmp_error__5;
+  struct asn_enc_rval_s tmp_error__6;
+  struct asn_enc_rval_s tmp_error__7;
+  int need_eom;
+  struct asn_enc_rval_s tmp_error__8;
+  struct asn_enc_rval_s tmp_error__9;
+  struct asn_enc_rval_s tmp_error__10;
+  register struct asn_INTEGER_specifics_s *$specs;
+  register struct ASN__PRIMITIVE_TYPE_s *$st;
+  register unsigned char *$buf;
+  register unsigned char *$end;
+  register struct asn_per_constraint_s *$ct;
+  register int $inext;
+  register int $mayEncode;
+  register int $355;
+  register int $354;
+  register int $353;
+  register int $352;
+  register int $351;
+  register int $350;
+  register int $349;
+  register int $348;
+  register int $347;
+  register int $346;
+  register int $345;
+  register int $344;
+  register int $343;
+  register int $342;
+  register void *$341;
+  register int $340;
+  register void *$386;
+  register unsigned int $385;
+  register int $384;
+  register int $383;
+  register unsigned int $382;
+  register int $381;
+  register unsigned int $380;
+  register int $379;
+  register unsigned int $378;
+  register int $377;
+  register int $376;
+  register unsigned int $375;
+  register int $374;
+  register int $373;
+  register int $372;
+  register int $371;
+  register int $370;
+  register int $369;
+  register int $368;
+  register int $367;
+  register int $366;
+  register int $365;
+  register int $364;
+  register int $363;
+  register int $362;
+  register int $361;
+  register unsigned int $360;
+  register int $359;
+  register unsigned int $358;
+  register unsigned char *$357;
+  register int $356;
+  $386 = (*$td).specifics;
+  $specs = (struct asn_INTEGER_specifics_s *) $386;
+  $st = (struct ASN__PRIMITIVE_TYPE_s *) $sptr;
+  value = 0;
+  if (!$st) {
+    $340 = 1;
+  } else {
+    $385 = (*$st).size;
+    $340 = (_Bool) ($385 == 0);
+  }
+  if ($340) {
+    for (; 1; ({ break; })) {
+      tmp_error.encoded = -1;
+      tmp_error.failed_type = $td;
+      tmp_error.structure_ptr = $sptr;
+      for (; 1; ({ break; })) {
+        /*skip*/;
+      }
+      *$_res = tmp_error;
+      return;
+    }
+  }
+  if (!$constraints) {
+    $constraints = (*$td).encoding_constraints.per_constraints;
+  }
+  if ($constraints) {
+    $341 = (void *) &(*$constraints).value;
+  } else {
+    $341 = (void *) (void *) 0;
+  }
+  $ct = $341;
+  er.encoded = 0;
+  if ($ct) {
+    $inext = 0;
+    if ($specs) {
+      $384 = (*$specs).field_unsigned;
+      $346 = (_Bool) $384;
+    } else {
+      $346 = 0;
+    }
+    if ($346) {
+      $342 = asn_INTEGER2ulong($st, &uval);
+      if ($342) {
+        for (; 1; ({ break; })) {
+          tmp_error__1.encoded = -1;
+          tmp_error__1.failed_type = $td;
+          tmp_error__1.structure_ptr = $sptr;
+          for (; 1; ({ break; })) {
+            /*skip*/;
+          }
+          *$_res = tmp_error__1;
+          return;
+        }
+      }
+      $376 = (*$ct).flags;
+      if ($376 & 1) {
+        $382 = uval;
+        $383 = (*$ct).lower_bound;
+        if ($382 < (unsigned int) $383) {
+          $inext = 1;
+        }
+      } else {
+        $377 = (*$ct).range_bits;
+        if ($377 >= 0) {
+          $378 = uval;
+          $379 = (*$ct).lower_bound;
+          if ($378 < (unsigned int) $379) {
+            $343 = 1;
+          } else {
+            $380 = uval;
+            $381 = (*$ct).upper_bound;
+            $343 = (_Bool) ($380 > (unsigned int) $381);
+          }
+          if ($343) {
+            $inext = 1;
+          }
+        }
+      }
+      for (; 1; ({ break; })) {
+        /*skip*/;
+      }
+      $375 = uval;
+      value = $375;
+    } else {
+      $344 = asn_INTEGER2long($st, &value);
+      if ($344) {
+        for (; 1; ({ break; })) {
+          tmp_error__2.encoded = -1;
+          tmp_error__2.failed_type = $td;
+          tmp_error__2.structure_ptr = $sptr;
+          for (; 1; ({ break; })) {
+            /*skip*/;
+          }
+          *$_res = tmp_error__2;
+          return;
+        }
+      }
+      $367 = (*$ct).flags;
+      if ($367 & 1) {
+        $373 = value;
+        $374 = (*$ct).lower_bound;
+        if ($373 < $374) {
+          $inext = 1;
+        }
+      } else {
+        $368 = (*$ct).range_bits;
+        if ($368 >= 0) {
+          $369 = value;
+          $370 = (*$ct).lower_bound;
+          if ($369 < $370) {
+            $345 = 1;
+          } else {
+            $371 = value;
+            $372 = (*$ct).upper_bound;
+            $345 = (_Bool) ($371 > $372);
+          }
+          if ($345) {
+            $inext = 1;
+          }
+        }
+      }
+      for (; 1; ({ break; })) {
+        /*skip*/;
+      }
+    }
+    $366 = (*$ct).flags;
+    if ($366 & 4) {
+      $347 = asn_put_few_bits($po, $inext, 1);
+      if ($347) {
+        for (; 1; ({ break; })) {
+          tmp_error__3.encoded = -1;
+          tmp_error__3.failed_type = $td;
+          tmp_error__3.structure_ptr = $sptr;
+          for (; 1; ({ break; })) {
+            /*skip*/;
+          }
+          *$_res = tmp_error__3;
+          return;
+        }
+      }
+      if ($inext) {
+        $ct = 0;
+      }
+    } else {
+      if ($inext) {
+        for (; 1; ({ break; })) {
+          tmp_error__4.encoded = -1;
+          tmp_error__4.failed_type = $td;
+          tmp_error__4.structure_ptr = $sptr;
+          for (; 1; ({ break; })) {
+            /*skip*/;
+          }
+          *$_res = tmp_error__4;
+          return;
+        }
+      }
+    }
+  }
+  if ($ct) {
+    $365 = (*$ct).range_bits;
+    $350 = (_Bool) ($365 >= 0);
+  } else {
+    $350 = 0;
+  }
+  if ($350) {
+    for (; 1; ({ break; })) {
+      /*skip*/;
+    }
+    $362 = value;
+    $363 = (*$ct).lower_bound;
+    $364 = (*$ct).upper_bound;
+    $348 = per_long_range_rebase($362, $363, $364, &v);
+    if ($348) {
+      for (; 1; ({ break; })) {
+        tmp_error__5.encoded = -1;
+        tmp_error__5.failed_type = $td;
+        tmp_error__5.structure_ptr = $sptr;
+        for (; 1; ({ break; })) {
+          /*skip*/;
+        }
+        *$_res = tmp_error__5;
+        return;
+      }
+    }
+    $360 = v;
+    $361 = (*$ct).range_bits;
+    $349 = uper_put_constrained_whole_number_u($po, $360, $361);
+    if ($349) {
+      for (; 1; ({ break; })) {
+        tmp_error__6.encoded = -1;
+        tmp_error__6.failed_type = $td;
+        tmp_error__6.structure_ptr = $sptr;
+        for (; 1; ({ break; })) {
+          /*skip*/;
+        }
+        *$_res = tmp_error__6;
+        return;
+      }
+    }
+    for (; 1; ({ break; })) {
+      er.structure_ptr = 0;
+      er.failed_type = 0;
+      *$_res = er;
+      return;
+    }
+  }
+  if ($ct) {
+    $359 = (*$ct).lower_bound;
+    $351 = (_Bool) $359;
+  } else {
+    $351 = 0;
+  }
+  if ($351) {
+    for (; 1; ({ break; })) {
+      /*skip*/;
+    }
+    for (; 1; ({ break; })) {
+      tmp_error__7.encoded = -1;
+      tmp_error__7.failed_type = $td;
+      tmp_error__7.structure_ptr = $sptr;
+      for (; 1; ({ break; })) {
+        /*skip*/;
+      }
+      *$_res = tmp_error__7;
+      return;
+    }
+  }
+  $buf = (*$st).buf;
+  $357 = (*$st).buf;
+  $358 = (*$st).size;
+  $end = $357 + $358;
+  while (1) {
+    if (! ($buf < $end)) {
+      break;
+    }
+    need_eom = 0;
+    $352 = uper_put_length($po, $end - $buf, &need_eom);
+    $mayEncode = $352;
+    if ($mayEncode < 0) {
+      for (; 1; ({ break; })) {
+        tmp_error__8.encoded = -1;
+        tmp_error__8.failed_type = $td;
+        tmp_error__8.structure_ptr = $sptr;
+        for (; 1; ({ break; })) {
+          /*skip*/;
+        }
+        *$_res = tmp_error__8;
+        return;
+      }
+    }
+    $353 = asn_put_many_bits($po, $buf, 8 * $mayEncode);
+    if ($353) {
+      for (; 1; ({ break; })) {
+        tmp_error__9.encoded = -1;
+        tmp_error__9.failed_type = $td;
+        tmp_error__9.structure_ptr = $sptr;
+        for (; 1; ({ break; })) {
+          /*skip*/;
+        }
+        *$_res = tmp_error__9;
+        return;
+      }
+    }
+    $buf = $buf + $mayEncode;
+    $356 = need_eom;
+    if ($356) {
+      $355 = uper_put_length($po, 0, 0);
+      $354 = (_Bool) $355;
+    } else {
+      $354 = 0;
+    }
+    if ($354) {
+      for (; 1; ({ break; })) {
+        tmp_error__10.encoded = -1;
+        tmp_error__10.failed_type = $td;
+        tmp_error__10.structure_ptr = $sptr;
+        for (; 1; ({ break; })) {
+          /*skip*/;
+        }
+        *$_res = tmp_error__10;
+        return;
+      }
+    }
+  }
+  for (; 1; ({ break; })) {
+    er.structure_ptr = 0;
+    er.failed_type = 0;
+    *$_res = er;
+    return;
+  }
+}
+
+long long asn__integer_convert(unsigned char *$b, unsigned char *$end)
+{
+  register unsigned long long $value;
+  register unsigned char $341;
+  register unsigned char $340;
+  $341 = *$b;
+  if ($341 >> 7) {
+    $value = (unsigned long long) -1;
+  } else {
+    $value = (unsigned long long) 0;
+  }
+  for (; 1; $b = $b + 1) {
+    if (! ($b < $end)) {
+      break;
+    }
+    $340 = *$b;
+    $value = $value << 8 | $340;
+  }
+  return $value;
+}
+
+int asn_INTEGER2imax(struct ASN__PRIMITIVE_TYPE_s *$iptr, long long *$lptr)
+{
+  register unsigned char *$b;
+  register unsigned char *$end;
+  register unsigned int $size;
+  register unsigned char *$end1;
+  register long long $344;
+  register int *$343;
+  register int $342;
+  register int $341;
+  register int *$340;
+  register unsigned char *$348;
+  register unsigned char $347;
+  register unsigned char $346;
+  register unsigned char $345;
+  if (!$iptr) {
+    $341 = 1;
+  } else {
+    $348 = (*$iptr).buf;
+    $341 = (_Bool) !$348;
+  }
+  if ($341) {
+    $342 = 1;
+  } else {
+    $342 = (_Bool) !$lptr;
+  }
+  if ($342) {
+    $340 = __errno_location();
+    *$340 = 22;
+    return -1;
+  }
+  $b = (*$iptr).buf;
+  $size = (*$iptr).size;
+  $end = $b + $size;
+  if ($size > sizeof(long long)) {
+    $end1 = $end - 1;
+    for (; 1; $b = $b + 1) {
+      if (! ($b < $end1)) {
+        break;
+      }
+      $345 = *$b;
+      switch ($345) {
+        case 0:
+          $347 = *($b + 1);
+          if (($347 & 128) == 0) {
+            continue;
+          }
+          break;
+        case 255:
+          $346 = *($b + 1);
+          if (($346 & 128) != 0) {
+            continue;
+          }
+          break;
+        
+      }
+      break;
+    }
+    $size = $end - $b;
+    if ($size > sizeof(long long)) {
+      $343 = __errno_location();
+      *$343 = 34;
+      return -1;
+    }
+  }
+  if ($end == $b) {
+    *$lptr = 0;
+    return 0;
+  }
+  $344 = asn__integer_convert($b, $end);
+  *$lptr = $344;
+  return 0;
+}
+
+int asn_INTEGER2umax(struct ASN__PRIMITIVE_TYPE_s *$iptr, unsigned long long *$lptr)
+{
+  register unsigned char *$b;
+  register unsigned char *$end;
+  register unsigned long long $value;
+  register unsigned int $size;
+  register int *$343;
+  register int $342;
+  register int $341;
+  register int *$340;
+  register unsigned char *$346;
+  register unsigned char $345;
+  register unsigned char $344;
+  if (!$iptr) {
+    $341 = 1;
+  } else {
+    $346 = (*$iptr).buf;
+    $341 = (_Bool) !$346;
+  }
+  if ($341) {
+    $342 = 1;
+  } else {
+    $342 = (_Bool) !$lptr;
+  }
+  if ($342) {
+    $340 = __errno_location();
+    *$340 = 22;
+    return -1;
+  }
+  $b = (*$iptr).buf;
+  $size = (*$iptr).size;
+  $end = $b + $size;
+  for (; 1; $b = $b + 1, $size = $size - 1) {
+    if (! ($size > sizeof(unsigned long long))) {
+      break;
+    }
+    $345 = *$b;
+    if ($345) {
+      $343 = __errno_location();
+      *$343 = 34;
+      return -1;
+    }
+  }
+  $value = (unsigned long long) 0;
+  for (; 1; $b = $b + 1) {
+    if (! ($b < $end)) {
+      break;
+    }
+    $344 = *$b;
+    $value = $value << 8 | $344;
+  }
+  *$lptr = $value;
+  return 0;
+}
+
+int asn_umax2INTEGER(struct ASN__PRIMITIVE_TYPE_s *$st, unsigned long long $value)
+{
+  register unsigned char *$buf;
+  register unsigned char *$end;
+  register unsigned char *$b;
+  register int $shr;
+  register void *$341;
+  register int $340;
+  register unsigned char *$343;
+  register unsigned char *$342;
+  if ($value <= ~((unsigned long long) 0) >> 1) {
+    $340 = asn_imax2INTEGER($st, $value);
+    return $340;
+  }
+  $341 = malloc(1 + sizeof(unsigned long long));
+  $buf = (unsigned char *) $341;
+  if (!$buf) {
+    return -1;
+  }
+  $end = $buf + (sizeof(unsigned long long) + 1);
+  *($buf + 0) = 0;
+  $b = $buf + 1;
+  $shr = (sizeof(unsigned long long) - 1) * 8;
+  for (; 1; $shr = $shr - 8, $b = $b + 1) {
+    if (! ($b < $end)) {
+      break;
+    }
+    *$b = (unsigned char) ($value >> $shr);
+  }
+  $342 = (*$st).buf;
+  if ($342) {
+    $343 = (*$st).buf;
+    free($343);
+  }
+  (*$st).buf = $buf;
+  (*$st).size = 1 + sizeof(unsigned long long);
+  return 0;
+}
+
+int asn_imax2INTEGER(struct ASN__PRIMITIVE_TYPE_s *$st, long long $value)
+{
+  long long value;
+  int littleEndian;
+  register unsigned char *$buf;
+  register unsigned char *$bp;
+  register unsigned char *$p;
+  register unsigned char *$pstart;
+  register unsigned char *$pend1;
+  register int $add;
+  register unsigned char *$342;
+  register void *$341;
+  register int *$340;
+  register signed char $349;
+  register unsigned char $348;
+  register unsigned char $347;
+  register unsigned char $346;
+  register unsigned char $345;
+  register unsigned char *$344;
+  register unsigned char *$343;
+  value = $value;
+  littleEndian = 1;
+  if (!$st) {
+    $340 = __errno_location();
+    *$340 = 22;
+    return -1;
+  }
+  $341 = malloc(sizeof(long long));
+  $buf = (unsigned char *) (int *) $341;
+  if (!$buf) {
+    return -1;
+  }
+  $349 = *((signed char *) &littleEndian);
+  if ($349) {
+    $pstart = (unsigned char *) &value + sizeof(long long) - 1;
+    $pend1 = (unsigned char *) &value;
+    $add = -1;
+  } else {
+    $pstart = (unsigned char *) &value;
+    $pend1 = $pstart + sizeof(long long) - 1;
+    $add = 1;
+  }
+  $p = $pstart;
+  for (; 1; $p = $p + $add) {
+    if (! ($p != $pend1)) {
+      break;
+    }
+    $346 = *$p;
+    switch ($346) {
+      case 0:
+        $348 = *($p + $add);
+        if (($348 & 128) == 0) {
+          continue;
+        }
+        break;
+      case 255:
+        $347 = *($p + $add);
+        if ($347 & 128) {
+          continue;
+        }
+        break;
+      
+    }
+    break;
+  }
+  $bp = $buf;
+  $pend1 = $pend1 + $add;
+  for (; 1; $p = $p + $add) {
+    if (! ($p != $pend1)) {
+      break;
+    }
+    $342 = $bp;
+    $bp = $342 + 1;
+    $345 = *$p;
+    *$342 = $345;
+  }
+  $343 = (*$st).buf;
+  if ($343) {
+    $344 = (*$st).buf;
+    free($344);
+  }
+  (*$st).buf = $buf;
+  (*$st).size = $bp - $buf;
+  return 0;
+}
+
+int asn_INTEGER2long(struct ASN__PRIMITIVE_TYPE_s *$iptr, int *$l)
+{
+  long long v;
+  register int $342;
+  register int $341;
+  register int *$340;
+  register long long $345;
+  register long long $344;
+  register long long $343;
+  $342 = asn_INTEGER2imax($iptr, &v);
+  if ($342 == 0) {
+    $344 = v;
+    if ($344 < -2147483647 - 1) {
+      $341 = 1;
+    } else {
+      $345 = v;
+      $341 = (_Bool) ($345 > 2147483647);
+    }
+    if ($341) {
+      $340 = __errno_location();
+      *$340 = 34;
+      return -1;
+    }
+    $343 = v;
+    *$l = $343;
+    return 0;
+  } else {
+    return -1;
+  }
+}
+
+int asn_INTEGER2ulong(struct ASN__PRIMITIVE_TYPE_s *$iptr, unsigned int *$l)
+{
+  unsigned long long v;
+  register int $341;
+  register int *$340;
+  register unsigned long long $343;
+  register unsigned long long $342;
+  $341 = asn_INTEGER2umax($iptr, &v);
+  if ($341 == 0) {
+    $343 = v;
+    if ($343 > 2147483647 * 2U + 1U) {
+      $340 = __errno_location();
+      *$340 = 34;
+      return -1;
+    }
+    $342 = v;
+    *$l = $342;
+    return 0;
+  } else {
+    return -1;
+  }
+}
+
+int asn_long2INTEGER(struct ASN__PRIMITIVE_TYPE_s *$st, int $value)
+{
+  register int $340;
+  $340 = asn_imax2INTEGER($st, $value);
+  return $340;
+}
+
+int asn_ulong2INTEGER(struct ASN__PRIMITIVE_TYPE_s *$st, unsigned int $value)
+{
+  register int $340;
+  $340 = asn_imax2INTEGER($st, $value);
+  return $340;
+}
+
+int asn_strtoimax_lim(signed char *$str, signed char **$end, long long *$intp)
+{
+  register int $sign;
+  register long long $value;
+  register long long $asn1_intmax_max;
+  register long long $upper_boundary;
+  register long long $last_digit_max;
+  register int $d;
+  register int $341;
+  register int $340;
+  register signed char *$351;
+  register signed char *$350;
+  register signed char $349;
+  register signed char *$348;
+  register signed char $347;
+  register signed char $346;
+  register signed char $345;
+  register signed char $344;
+  register signed char $343;
+  register signed char *$342;
+  $sign = 1;
+  $asn1_intmax_max = ~((unsigned long long) 0) >> 1;
+  $upper_boundary = $asn1_intmax_max / 10;
+  $last_digit_max = $asn1_intmax_max % 10;
+  $351 = *$end;
+  if ($str >= $351) {
+    return -2;
+  }
+  $349 = *$str;
+  switch ($349) {
+    case 45:
+      $last_digit_max = $last_digit_max + 1;
+      $sign = -1;
+    case 43:
+      $str = $str + 1;
+      $350 = *$end;
+      if ($str >= $350) {
+        *$end = $str;
+        return -1;
+      }
+    
+  }
+  $value = (long long) 0;
+  for (; 1; $str = $str + 1) {
+    $348 = *$end;
+    if (! ($str < $348)) {
+      break;
+    }
+    $346 = *$str;
+    if ($346 >= 48) {
+      $347 = *$str;
+      $341 = (_Bool) ($347 <= 57);
+    } else {
+      $341 = 0;
+    }
+    if ($341) {
+      $345 = *$str;
+      $d = $345 - 48;
+      if ($value < $upper_boundary) {
+        $value = $value * 10 + $d;
+      } else {
+        if ($value == $upper_boundary) {
+          if ($d <= $last_digit_max) {
+            if ($sign > 0) {
+              $value = $value * 10 + $d;
+            } else {
+              $sign = 1;
+              $value = -$value * 10 - $d;
+            }
+            $str = $str + 1;
+            $342 = *$end;
+            if ($str < $342) {
+              *$end = $str;
+              $343 = *$str;
+              if ($343 >= 48) {
+                $344 = *$str;
+                $340 = (_Bool) ($344 <= 57);
+              } else {
+                $340 = 0;
+              }
+              if ($340) {
+                return -3;
+              } else {
+                *$intp = $sign * $value;
+                return 1;
+              }
+            }
+            break;
+          } else {
+            *$end = $str;
+            return -3;
+          }
+        } else {
+          *$end = $str;
+          return -3;
+        }
+      }
+    } else {
+      *$end = $str;
+      *$intp = $sign * $value;
+      return 1;
+    }
+  }
+  *$end = $str;
+  *$intp = $sign * $value;
+  return 0;
+}
+
+int asn_strtoumax_lim(signed char *$str, signed char **$end, unsigned long long *$uintp)
+{
+  register unsigned long long $value;
+  register unsigned long long $asn1_uintmax_max;
+  register unsigned long long $upper_boundary;
+  register unsigned long long $last_digit_max;
+  register unsigned int $d;
+  register int $341;
+  register int $340;
+  register signed char *$351;
+  register signed char *$350;
+  register signed char $349;
+  register signed char *$348;
+  register signed char $347;
+  register signed char $346;
+  register signed char $345;
+  register signed char $344;
+  register signed char $343;
+  register signed char *$342;
+  $asn1_uintmax_max = ~((unsigned long long) 0);
+  $upper_boundary = $asn1_uintmax_max / 10;
+  $last_digit_max = $asn1_uintmax_max % 10;
+  $351 = *$end;
+  if ($str >= $351) {
+    return -2;
+  }
+  $349 = *$str;
+  switch ($349) {
+    case 45:
+      return -2;
+    case 43:
+      $str = $str + 1;
+      $350 = *$end;
+      if ($str >= $350) {
+        *$end = $str;
+        return -1;
+      }
+    
+  }
+  $value = (unsigned long long) 0;
+  for (; 1; $str = $str + 1) {
+    $348 = *$end;
+    if (! ($str < $348)) {
+      break;
+    }
+    $346 = *$str;
+    if ($346 >= 48) {
+      $347 = *$str;
+      $341 = (_Bool) ($347 <= 57);
+    } else {
+      $341 = 0;
+    }
+    if ($341) {
+      $345 = *$str;
+      $d = $345 - 48;
+      if ($value < $upper_boundary) {
+        $value = $value * 10 + $d;
+      } else {
+        if ($value == $upper_boundary) {
+          if ($d <= $last_digit_max) {
+            $value = $value * 10 + $d;
+            $str = $str + 1;
+            $342 = *$end;
+            if ($str < $342) {
+              *$end = $str;
+              $343 = *$str;
+              if ($343 >= 48) {
+                $344 = *$str;
+                $340 = (_Bool) ($344 <= 57);
+              } else {
+                $340 = 0;
+              }
+              if ($340) {
+                return -3;
+              } else {
+                *$uintp = $value;
+                return 1;
+              }
+            }
+            break;
+          } else {
+            *$end = $str;
+            return -3;
+          }
+        } else {
+          *$end = $str;
+          return -3;
+        }
+      }
+    } else {
+      *$end = $str;
+      *$uintp = $value;
+      return 1;
+    }
+  }
+  *$end = $str;
+  *$uintp = $value;
+  return 0;
+}
+
+signed char const __func__[15] = { 97, 115, 110, 95, 115, 116, 114, 116, 111,
+  108, 95, 108, 105, 109, 0, };
+
+int asn_strtol_lim(signed char *$str, signed char **$end, int *$lp)
+{
+  long long value;
+  register int $342;
+  register int $341;
+  register int $340;
+  register long long $348;
+  register long long $347;
+  register long long $346;
+  register long long $345;
+  register long long $344;
+  register long long $343;
+  $340 = asn_strtoimax_lim($str, $end, &value);
+  switch ($340) {
+    case 4294967293:
+      return -3;
+    case 4294967294:
+      return -2;
+    case 4294967295:
+      return -1;
+    case 0:
+      $347 = value;
+      if ($347 >= -2147483647 - 1) {
+        $348 = value;
+        $341 = (_Bool) ($348 <= 2147483647);
+      } else {
+        $341 = 0;
+      }
+      if ($341) {
+        $346 = value;
+        *$lp = $346;
+        return 0;
+      } else {
+        return -3;
+      }
+    case 1:
+      $344 = value;
+      if ($344 >= -2147483647 - 1) {
+        $345 = value;
+        $342 = (_Bool) ($345 <= 2147483647);
+      } else {
+        $342 = 0;
+      }
+      if ($342) {
+        $343 = value;
+        *$lp = $343;
+        return 1;
+      } else {
+        return -3;
+      }
+    
+  }
+  if (! !__stringlit_10) {
+    __assert_fail(__stringlit_9, __stringlit_8, 1195, __func__);
+  }
+  return -2;
+}
+
+signed char const __func____1[16] = { 97, 115, 110, 95, 115, 116, 114, 116,
+  111, 117, 108, 95, 108, 105, 109, 0, };
+
+int asn_strtoul_lim(signed char *$str, signed char **$end, unsigned int *$ulp)
+{
+  unsigned long long value;
+  register int $340;
+  register unsigned long long $344;
+  register unsigned long long $343;
+  register unsigned long long $342;
+  register unsigned long long $341;
+  $340 = asn_strtoumax_lim($str, $end, &value);
+  switch ($340) {
+    case 4294967293:
+      return -3;
+    case 4294967294:
+      return -2;
+    case 4294967295:
+      return -1;
+    case 0:
+      $343 = value;
+      if ($343 <= 2147483647 * 2U + 1U) {
+        $344 = value;
+        *$ulp = $344;
+        return 0;
+      } else {
+        return -3;
+      }
+    case 1:
+      $341 = value;
+      if ($341 <= 2147483647 * 2U + 1U) {
+        $342 = value;
+        *$ulp = $342;
+        return 1;
+      } else {
+        return -3;
+      }
+    
+  }
+  if (! !__stringlit_10) {
+    __assert_fail(__stringlit_9, __stringlit_8, 1225, __func____1);
+  }
+  return -2;
+}
+
+int INTEGER_compare(struct asn_TYPE_descriptor_s *$td, void *$aptr, void *$bptr)
+{
+  register struct ASN__PRIMITIVE_TYPE_s *$a;
+  register struct ASN__PRIMITIVE_TYPE_s *$b;
+  register int $sign_a;
+  register int $sign_b;
+  register int $sign;
+  register int $sign__1;
+  register int $347;
+  register int $346;
+  register int $345;
+  register int $344;
+  register int $343;
+  register int $342;
+  register int $341;
+  register int $340;
+  register unsigned int $366;
+  register unsigned int $365;
+  register unsigned char $364;
+  register unsigned char *$363;
+  register unsigned char $362;
+  register unsigned char *$361;
+  register unsigned int $360;
+  register unsigned int $359;
+  register unsigned int $358;
+  register unsigned int $357;
+  register unsigned int $356;
+  register unsigned char *$355;
+  register unsigned char *$354;
+  register unsigned char $353;
+  register unsigned char *$352;
+  register unsigned char $351;
+  register unsigned char *$350;
+  register unsigned int $349;
+  register unsigned int $348;
+  $a = $aptr;
+  $b = $bptr;
+  if ($a) {
+    $347 = (_Bool) $b;
+  } else {
+    $347 = 0;
+  }
+  if ($347) {
+    $365 = (*$a).size;
+    if ($365) {
+      $366 = (*$b).size;
+      $345 = (_Bool) $366;
+    } else {
+      $345 = 0;
+    }
+    if ($345) {
+      $363 = (*$a).buf;
+      $364 = *($363 + 0);
+      if ($364 & 128) {
+        $340 = (int) -1;
+      } else {
+        $340 = (int) 1;
+      }
+      $sign_a = $340;
+      $361 = (*$b).buf;
+      $362 = *($361 + 0);
+      if ($362 & 128) {
+        $341 = (int) -1;
+      } else {
+        $341 = (int) 1;
+      }
+      $sign_b = $341;
+      if ($sign_a < $sign_b) {
+        return -1;
+      }
+      if ($sign_a > $sign_b) {
+        return 1;
+      }
+      $357 = (*$a).size;
+      $358 = (*$b).size;
+      if ($357 < $358) {
+        return -1 * $sign_a;
+      } else {
+        $359 = (*$a).size;
+        $360 = (*$b).size;
+        if ($359 > $360) {
+          return 1 * $sign_b;
+        }
+      }
+      $354 = (*$a).buf;
+      $355 = (*$b).buf;
+      $356 = (*$a).size;
+      $342 = memcmp($354, $355, $356);
+      return $sign_a * $342;
+    } else {
+      $348 = (*$a).size;
+      if ($348) {
+        $352 = (*$a).buf;
+        $353 = *($352 + 0);
+        if ($353 & 128) {
+          $343 = (int) -1;
+        } else {
+          $343 = (int) 1;
+        }
+        $sign = $343;
+        return 1 * $sign;
+      } else {
+        $349 = (*$b).size;
+        if ($349) {
+          $350 = (*$a).buf;
+          $351 = *($350 + 0);
+          if ($351 & 128) {
+            $344 = (int) -1;
+          } else {
+            $344 = (int) 1;
+          }
+          $sign__1 = $344;
+          return -1 * $sign__1;
+        } else {
+          return 0;
+        }
+      }
+    }
+  } else {
+    if (!$a) {
+      $346 = (_Bool) !$b;
+    } else {
+      $346 = 0;
+    }
+    if ($346) {
+      return 0;
+    } else {
+      if (!$a) {
+        return -1;
+      } else {
+        return 1;
+      }
+    }
+  }
+}
+
+signed char const __func____2[20] = { 73, 78, 84, 69, 71, 69, 82, 95, 114,
+  97, 110, 100, 111, 109, 95, 102, 105, 108, 108, 0, };
+
+int const variants[38] = { -65536, -65535, -65534, -32769, -32768, -32767,
+  -16385, -16384, -16383, -257, -256, -255, -254, -129, -128, -127, -126, -1,
+  0, 1, 126, 127, 128, 129, 254, 255, 256, 257, 16383, 16384, 16385, 32767,
+  32768, 32769, 65534, 65535, 65536, 65537, };
+
+void INTEGER_random_fill(struct asn_random_fill_result_s *$_res, struct asn_TYPE_descriptor_s *$td, void **$sptr, struct asn_encoding_constraints_s *$constraints, unsigned int $max_length)
+{
+  struct asn_random_fill_result_s result_ok;
+  struct asn_random_fill_result_s result_failed;
+  struct asn_random_fill_result_s result_skipped;
+  register struct asn_INTEGER_specifics_s *$specs;
+  register struct ASN__PRIMITIVE_TYPE_s *$st;
+  register struct asn_INTEGER_enum_map_s *$emap;
+  register unsigned int $emap_len;
+  register long long $value;
+  register int $find_inside_map;
+  register struct asn_per_constraints_s *$ct;
+  register int $351;
+  register int $350;
+  register int $349;
+  register long long $348;
+  register void *$347;
+  register int $346;
+  register long long $345;
+  register long long $344;
+  register long long $343;
+  register long long $342;
+  register long long $341;
+  register void *$340;
+  register void *$370;
+  register int $369;
+  register int $368;
+  register int $367;
+  register int $366;
+  register int $365;
+  register int $364;
+  register struct asn_per_constraints_s *$363;
+  register int $362;
+  register int $361;
+  register int $360;
+  register int $359;
+  register int $358;
+  register void (*$357)(struct asn_TYPE_descriptor_s *, void *, int);
+  register struct asn_TYPE_operation_s *$356;
+  register void (*$355)(struct asn_TYPE_descriptor_s *, void *, int);
+  register struct asn_TYPE_operation_s *$354;
+  register void *$353;
+  register unsigned int $352;
+  $370 = (*$td).specifics;
+  $specs = (struct asn_INTEGER_specifics_s *) $370;
+  result_ok.code = 0;
+  result_ok.length = 1;
+  result_failed.code = -1;
+  result_failed.length = 0;
+  result_skipped.code = 1;
+  result_skipped.length = 0;
+  $st = *$sptr;
+  if ($max_length == 0) {
+    *$_res = result_skipped;
+    return;
+  }
+  if ($st == (void *) 0) {
+    $340 = calloc(1, sizeof(struct ASN__PRIMITIVE_TYPE_s));
+    $st = (struct ASN__PRIMITIVE_TYPE_s *) $340;
+    if ($st == (void *) 0) {
+      *$_res = result_failed;
+      return;
+    }
+  }
+  if ($specs) {
+    $emap = (*$specs).value2enum;
+    $emap_len = (*$specs).map_count;
+    $369 = (*$specs).strict_enumeration;
+    if ($369) {
+      $find_inside_map = $emap_len > 0;
+    } else {
+      if ($emap_len) {
+        $342 = asn_random_between(0, 1);
+        $341 = (long long) $342;
+      } else {
+        $341 = (long long) 0;
+      }
+      $find_inside_map = (int) $341;
+    }
+  } else {
+    $emap = 0;
+    $emap_len = 0;
+    $find_inside_map = 0;
+  }
+  if ($find_inside_map) {
+    if (! ($emap_len > 0)) {
+      __assert_fail(__stringlit_12, __stringlit_8, 1311, __func____2);
+    }
+    $343 = asn_random_between(0, $emap_len - 1);
+    $368 = (*($emap + $343)).nat_value;
+    $value = (long long) $368;
+  } else {
+    if ($specs) {
+      $367 = (*$specs).field_unsigned;
+      $346 = (_Bool) $367;
+    } else {
+      $346 = 0;
+    }
+    if ($346) {
+      $366 = *(variants + 18);
+      if (! ($366 == 0)) {
+        __assert_fail(__stringlit_11, __stringlit_8, 1323, __func____2);
+      }
+      $344 = asn_random_between(18, sizeof(int [38]) / sizeof(int) - 1);
+      $365 = *(variants + $344);
+      $value = (long long) $365;
+    } else {
+      $345 = asn_random_between(0, sizeof(int [38]) / sizeof(int) - 1);
+      $364 = *(variants + $345);
+      $value = (long long) $364;
+    }
+    if (!$constraints) {
+      $constraints = &(*$td).encoding_constraints;
+    }
+    if ($constraints) {
+      $363 = (*$constraints).per_constraints;
+      $347 = (void *) $363;
+    } else {
+      $347 = (void *) (void *) 0;
+    }
+    $ct = $347;
+    if ($ct) {
+      $362 = (*$ct).value.flags;
+      $350 = (_Bool) ($362 & 2);
+    } else {
+      $350 = 0;
+    }
+    if ($350) {
+      $360 = (*$ct).value.lower_bound;
+      if ($value < $360) {
+        $349 = 1;
+      } else {
+        $361 = (*$ct).value.upper_bound;
+        $349 = (_Bool) ($value > $361);
+      }
+      if ($349) {
+        $358 = (*$ct).value.lower_bound;
+        $359 = (*$ct).value.upper_bound;
+        $348 = asn_random_between($358, $359);
+        $value = $348;
+      }
+    }
+  }
+  $351 = asn_imax2INTEGER($st, $value);
+  if ($351) {
+    $353 = *$sptr;
+    if ($st == $353) {
+      $356 = (*$td).op;
+      $357 = (*$356).free_struct;
+      $357($td, $st, 2);
+    } else {
+      $354 = (*$td).op;
+      $355 = (*$354).free_struct;
+      $355($td, $st, 0);
+    }
+    *$_res = result_failed;
+    return;
+  } else {
+    *$sptr = $st;
+    $352 = (*$st).size;
+    result_ok.length = $352;
+    *$_res = result_ok;
+    return;
+  }
+}
+
+
